full compiler correctness thm (with cheats)

compiler/compilerScript.sml
@@ -1,11 +1,54 @@
-open HolKernel boolLib bossLib l1_to_il1_compilerTheory il1_to_il2_compilerTheory store_creationTheory il1_il2_correctnessTheory l1_il1_correctnessTheory lcsymtacs;
+open HolKernel boolLib bossLib l1_to_il1_compilerTheory il1_to_il2_compilerTheory store_creationTheory il1_il2_correctnessTheory l1_il1_correctnessTheory lcsymtacs il2_to_il3_compilerTheory listTheory;
 
 val _ = new_theory "compiler"
 
-val compile_def = Define `compile e = il1_to_il2 (l1_to_il1 e 0)`;
+val compile_il2_def = Define `compile_il2 e = il1_to_il2 (l1_to_il1 e 0)`;
+
+val compile_def = Define `compile e = il2_to_il3 (compile_il2 e)`;
+
+val ms_il2_st_thm = prove(``!e.ms_il2 e (create_il2_store e)``, cheat)
+
+val il2_equiv_thm = prove(``!e st1 pc v st1' st2. exec (compile_il2 e) (0, [], st1) (pc, [v], st1') /\ equiv st1 st2 ==> ?st2'.
+exec (compile_il2 e) (0, [], st2) (pc, [v], st2') /\ equiv st1' st2'``, cheat);
+
+val store_equiv_gen_thm = prove(``!e.equiv (con_store (create_store e)) (create_il2_store (compile_il2 e))``, cheat);
 
 val TOTAL_CORRECTNESS_THM = store_thm("TOTAL_CORRECTNESS_THM",
-``!e v s'.bs_l1 (e, create_store e) v s' ==> ?pc' s''.exec (compile e) (0, [], con_store (create_store e)) (pc', [(il1_il2_val (l1_il1_val v))], s'')``,
-metis_tac [compile_def, L1_TO_IL1_EXISTS_CORRECTNESS_THM, CORRECTNESS_THM]);
+``!e v s'.bs_l1 (e, create_store e) v s' ==> ?s''.exec (compile_il2 e) (0, [], con_store (create_store e)) (&LENGTH (compile_il2 e), [(il1_il2_val (l1_il1_val v))], s'')``,
+metis_tac [compile_il2_def, L1_TO_IL1_EXISTS_CORRECTNESS_THM, CORRECTNESS_THM]);
+
+val length_prog_thm = prove(``!e.LENGTH (compile e) = LENGTH (compile_il2 e)``, rw [compile_def, compile_il2_def, il2_to_il3_def]);
+
+val create_il2_store_def = Define `
+(create_il2_store [] = FEMPTY) /\
+(create_il2_store (IL2_Store l::xs) = (create_il2_store xs) |+ (l, 0)) /\
+(create_il2_store (IL2_Load l::xs) = (create_il2_store xs) |+ (l, 0)) /\
+(create_il2_store (_::xs) = (create_il2_store xs))`;
+
+val make_stack_def = Define `make_stack e = astack (compile e)
+            (MAP_KEYS (map_fun (FST (make_loc_map (compile_il2 e))))
+               (create_il2_store (compile_il2 e))) []`;
+
+val total_c_lem = prove(``!e v s'.
+    bs_l1 (e, create_store e) v s' ==> 
+    ?astk.
+        vsm_exec (compile e) (0, make_stack e) (&LENGTH (compile e), (il1_il2_val (l1_il1_val v))::astk)``,
+
+rw [make_stack_def]
+
+THEN imp_res_tac TOTAL_CORRECTNESS_THM
+
+THEN `equiv (con_store (create_store e)) (create_il2_store (compile_il2 e))` by metis_tac [store_equiv_gen_thm]
+
+THEN imp_res_tac il2_equiv_thm
+
+THEN `ms_il2 (compile_il2 e) (create_il2_store (compile_il2 e))` by metis_tac [ms_il2_st_thm]
+
+THEN imp_res_tac il2_vsm_correctness
+
+THEN `?atsk.astk''' = (il1_il2_val (l1_il1_val v))::atsk` by (Cases_on `astk'''` THEN fs [TAKE_def]
+THEN Cases_on `n''' = 0` THEN fs [])
+
+THEN metis_tac [compile_def, length_prog_thm]);
 
 val _ = export_theory ();
